more on open graphs

coq/open.v
@@ -11,6 +11,14 @@ Unset Strict Implicit.
 Unset Printing Implicit Defensive.
 Set Bullet Behavior "Strict Subproofs". 
 
+Open Scope fset_scope.
+
+Require Import confluence.
+
+(** For the sake of clarity, we define two aliases of [nat], the type
+[VT] of graph vertices and the type [ET] of graph edges. For each type
+we have an injection into the type from any finite type via the rank
+of the element in the enumeration (i.e., [enum_rank]) *)
 
 Definition VT := nat.
 Definition ET := nat.
@@ -29,6 +37,48 @@ Lemma inj_e_inj : injective inj_e.
 Proof. move => x y. by move/ord_inj/enum_rank_inj. Qed.
 End inject.
 
+
+Definition fresh (E : {fset ET}) : ET := (\max_(e <- E) e).+1.
+
+Lemma freshP (E : {fset ET}) : fresh E \in E = false. 
+Proof. Admitted.
+
+(** Bijection between a finite type and the image of its injection into an arbitarty choiceType *)
+Lemma in_imfsetT (aT : finType) (rT : choiceType) (f : aT -> rT) (x : aT) : 
+  f x \in [fset f x | x in aT].
+Proof. by rewrite in_imfset. Qed.
+
+Lemma imfset_inv (aT : finType) (rT : choiceType) (f : aT -> rT) (y : [fset f x | x in aT]) : 
+  Σ x : aT, f x = val y.
+Proof. 
+  suff E : exists x, f x == val y by exists (xchoose E); rewrite (eqP (xchooseP E)).
+  case/imfsetP : (valP y) => /= x _ ->. by exists x.
+Qed.
+
+Section Bij.
+Variable (G : finType) (T : choiceType) (g : G -> T).
+Hypothesis g_inj : injective g.
+Let vset := [fset g x | x in G].
+Let f (x : G) : vset := Sub (g x) (in_imfsetT g x).
+Let f_inv (x : vset) : G := tag (imfset_inv x).
+
+Lemma can_vset : cancel f f_inv.
+Proof. 
+  move => x. rewrite /f_inv /f /=. set S := Sub _ _. 
+  apply: g_inj. by rewrite (tagged (imfset_inv S)).
+Qed.
+
+Lemma can_vset' : cancel f_inv f.
+Proof.
+  move => [x Hx]. rewrite /f /f_inv. apply: val_inj => /=.
+  by rewrite (tagged (imfset_inv [` Hx])).
+Qed.
+
+Definition imfset_bij := Bij can_vset can_vset'.
+End Bij.
+
+(** * Open Graphs *)
+
 Record pre_graph := { vset : {fset VT};
                       eset : {fset ET};
                       src : ET -> VT;
@@ -44,7 +94,7 @@ Class is_graph (G : pre_graph) :=
     p_inP : p_in G \in vset G;
     p_outP : p_out G \in vset G}.
 
-Open Scope fset_scope.
+(** ** Opening and closing of type-based graphs *)
 
 Section Open.
 Variable (G : lgraph).
@@ -60,6 +110,7 @@ Proof.
   case: insubP => [k _ /ord_inj -> /=|]; by rewrite ?P ?enum_rankK.
 Qed.
 
+(** For two-pointed graphs, we can use the input as default vertex when inverting the injection into [VT] *)
 Definition proj_v (v : VT) : G :=
   odflt input (omap enum_val (insub v : option 'I_#|G|)).
 
@@ -96,10 +147,10 @@ Variable (G : pre_graph).
 Context {graph_G : is_graph G}.
 
 Lemma source_proof (e : eset G) : src G (val e) \in vset G.
-Admitted.
+Proof. exact: (srcP (valP e)). Qed.
 
 Lemma target_proof (e : eset G) : tgt G (val e) \in vset G.
-Admitted.
+Proof. exact: (tgtP (valP e)). Qed.
 
 Definition close' : graph test_setoid term_setoid := Eval simpl in 
   {| vertex := [finType of vset G];
@@ -120,35 +171,6 @@ Notation "'Σ' x .. y , p" :=
   (sigT (fun x => .. (sigT (fun y => p%type)) ..))
   (at level 200, x binder, y binder, right associativity).
 
-Lemma in_imfsetT (aT : finType) (rT : choiceType) (f : aT -> rT) (x : aT) : 
-  f x \in [fset f x | x in aT].
-Proof. by rewrite in_imfset. Qed.
-
-Lemma imfset_inv (aT : finType) (rT : choiceType) (f : aT -> rT) (y : [fset f x | x in aT]) : 
-  Σ x : aT, f x = val y.
-Admitted.
-
-Section Bij.
-Variable (G : finType) (T : choiceType) (g : G -> T).
-Hypothesis g_inj : injective g.
-Let vset := [fset g x | x in G].
-Let f (x : G) : vset := Sub (g x) (in_imfsetT g x).
-Let f_inv (x : vset) : G := tag (imfset_inv x).
-
-Lemma can_vset : cancel f f_inv.
-Proof. 
-  move => x. rewrite /f_inv /f /=. set S := Sub _ _. 
-  apply: g_inj. by rewrite (tagged (imfset_inv S)).
-Qed.
-
-Lemma can_vset' : cancel f_inv f.
-Proof.
-  move => [x Hx]. rewrite /f /f_inv. apply: val_inj => /=.
-  by rewrite (tagged (imfset_inv [` Hx])).
-Qed.
-
-Definition imfset_bij := Bij can_vset can_vset'.
-End Bij.
 
 Lemma openK (G : lgraph) : G ≅ close (open G). 
 liso (imfset_bij (@inj_v_inj G)) 
@@ -161,6 +183,8 @@ liso (imfset_bij (@inj_v_inj G))
 - exact: val_inj.
 - exact: val_inj.
 Defined.
+
+(** We define isomorphisms via closing *)
 
 Definition oliso (G H : pre_graph) :=
   Σ (graph_G : is_graph G) (graph_H : is_graph H), close G ≅ close H.
@@ -180,6 +204,10 @@ Proof.
   apply: liso_comp I. exact: close_irrelevance.
 Qed.
 
+Lemma closeK (G : pre_graph) (graph_G : is_graph G) : 
+  G ⩭ open (close G).
+Proof. rewrite /oliso. do 2 eexists. exact: openK. Defined.
+
 
 Section PreGraphOps.
 Variables (G : pre_graph).
@@ -187,7 +215,6 @@ Variables (G : pre_graph).
 Definition incident x e := (src G e == x) || (tgt G e == x).
 
 Definition edges_at x := [fset e in eset G | incident x e].
-
 
 End PreGraphOps.
 
@@ -201,15 +228,36 @@ Definition del_vertex (G : pre_graph) (x : VT) :=
      p_in := p_in G;
      p_out := p_out G |}.
 
-Definition IO (G : pre_graph) := [fset p_in G; p_out G].
+Definition pIO (G : pre_graph) := [fset p_in G; p_out G].
 
 Notation "G \ x" := (del_vertex G x) (at level 25,left associativity).
 
-Global Instance del_vertex_graph (G : pre_graph) {graph_G : is_graph G} (x : VT) {Hx : x \notin IO G} : 
+Lemma edges_atF G e x : 
+  e \notin edges_at G x -> (src G e == x = false)*(tgt G e == x = false).
+Admitted.
+
+Lemma pIO_Ni  (G : pre_graph) x : x \notin pIO G -> p_in G != x.
+Admitted.
+
+Lemma pIO_No  (G : pre_graph) x : x \notin pIO G -> p_out G != x.
+Admitted.
+
+
+(** Experimental: A class of boxed properties to allow inference of "non-class" assumptions *)
+Class box (P : Prop) : Prop := Box { boxed : P }.
+Hint Extern 0 (box _) => apply Box; assumption : typeclass_instances.
+
+Global Instance del_vertex_graph (G : pre_graph) `{graph_G : is_graph G} (x : VT) `{Hx : box (x \notin pIO G)} : 
   is_graph (del_vertex G x).
 Proof.
   rewrite /del_vertex; split => //=. 
-Admitted.
+  - move => e /fsetDP [/srcP A B]. by rewrite !inE A edges_atF.
+  - move => e /fsetDP [/tgtP A B]. by rewrite !inE A edges_atF.
+  - case: Hx => Hx. by rewrite !inE p_inP andbT pIO_Ni.
+  - case: Hx => Hx. by rewrite !inE p_outP andbT pIO_No.
+Qed.
+
+Fail Fail Goal (forall (G : pre_graph) (graph_G : is_graph G) x (Hx : x \notin pIO G), close (G \ x)).
 
 Lemma edges_at_del (G : pre_graph) (z x : VT) : 
   edges_at (G \ z) x = edges_at G x `\` edges_at G z.
@@ -225,6 +273,221 @@ Proof.
   - by rewrite !edges_at_del fsetDDD fsetUC -fsetDDD.
 Qed.
 
+Definition del_edges (G : pre_graph) (E : {fset ET}) := 
+  {| vset := vset G;
+     eset := eset G `\` E;
+     src := src G;
+     tgt := tgt G;
+     lv := lv G;
+     le := le G;
+     p_in := p_in G;
+     p_out := p_out G |}.
+
+Global Instance del_edges_graph (G : pre_graph) `{graph_G : is_graph G} (E : {fset ET}) :
+  is_graph (del_edges G E).
+Admitted.
+
+Arguments fset1Ur [K x a B].
+Arguments fset1U1 [K x B].
+Arguments fset1U1 [K x B].
+
+Lemma fresh_eqF (E : {fset ET}) (x : E) : val x == fresh E = false.
+Admitted.
+
+Lemma valK' (T : Type) (P : pred T) (sT : subType P) (x : sT) (p : P (val x)) : 
+  Sub (val x) p = x.
+Proof. apply: val_inj. by rewrite SubK. Qed.
+
+(* TODO: generalize to any [e \notin E] *)
+Lemma fresh_bij (T : finType) (E : {fset ET}) (f : bij T E) : bij (option T) (fresh E |` E).
+Proof.
+  pose g (x : option T) : fresh E |` E := 
+    if x is Some z then Sub (val (f z)) (fset1Ur (valP (f z))) else Sub (fresh E) fset1U1.
+  pose g_inv  (x : fresh E |` E) : option T := 
+    match fsetULVR (valP x) with inl _ => None | inr p => Some (f^-1 (Sub (val x) p)) end.
+  have can_g : cancel g g_inv.
+  { move => [x|]; rewrite /g/g_inv/=; case: (fsetULVR _) => [|p] //=. 
+    - by rewrite inE fresh_eqF.
+    - by rewrite valK' bijK.
+    - exfalso. by rewrite freshP in p. }
+  have can_g_inv : cancel g_inv g.
+  { move => [x Hx]; rewrite /g/g_inv/=. case: (fsetULVR _) => [|p] //=. 
+    - rewrite !inE => A. apply: val_inj => /=. by rewrite (eqP A).
+    - apply: val_inj => //=. by rewrite bijK'. }
+  apply: (Bij can_g can_g_inv).
+Defined.
+
+Lemma fresh_bijE (T : finType) (E : {fset ET}) (f : bij T E) : 
+  (forall x, fresh_bij f (Some x) = Sub (val (f x)) (fset1Ur (valP (f x))))*
+  (fresh_bij f None = Sub (fresh E) fset1U1).
+Proof. done. Qed.
+
+Definition update (aT : eqType) (rT : Type) (f : aT -> rT) x y := 
+  fun z => if z == x then y else f z.
+(* Notation "f [ x := y ]" := (update f x y) (at level 2, format "f [ x  :=  y ]"). *)
+
+Definition add_edge (G : pre_graph) x u y :=
+  let e := fresh (eset G) in
+  {| vset := vset G;
+     eset := e |` eset G;
+     src := update (src G) e x;
+     tgt := update (tgt G) e y;
+     lv := lv G;
+     le := update (le G) e u;
+     p_in := p_in G;
+     p_out := p_out G |}.
+
+(* TOTHINK: This is not an instance because [x \in vset G] is not
+inferrable. One could box it though and make it inferrable through
+some external hints *)
+Lemma add_edge_graph (G : pre_graph) (graph_G : is_graph G) x y u :
+  x \in vset G -> y \in vset G -> is_graph (add_edge G x u y).
+Admitted.
+
+Definition add_test (G : pre_graph) (x:VT) (a:test) := 
+  {| vset := vset G;
+     eset := eset G;
+     src := src G;
+     tgt := tgt G;
+     lv := update (lv G) x [lv G x·a];
+     le := le G;
+     p_in := p_in G;
+     p_out := p_out G |}.
+
+Definition oarc (G : pre_graph) e x u y := 
+  [/\ src G e = x, tgt G e = y & le G e ≡ u] \/
+  [/\ tgt G e = x, src G e = y & le G e ≡ u°].
+
+Inductive ostep : pre_graph -> pre_graph -> Type := 
+  ostep_v1 (G : pre_graph) x z e u : 
+    Top.edges_at G z = [fset e] -> z \notin pIO G -> oarc G e x u z -> x != z ->
+    ostep G (add_test G  x [dom(u·lv G z)] \ z).
+
+Section Transfer.
+Variable (G : lgraph).
+
+Lemma fresh_imfsetF (T : finType) (f : T -> ET) (e : T) :
+   f e == fresh [fset f x | x in T] = false.
+Admitted. 
+
+Lemma inj_v_open (x : G) : inj_v x \in vset (open G).
+Proof. by rewrite in_imfset. Qed.
+Hint Resolve inj_v_open.
+
+Lemma open_add_edge (x y : G) u : 
+  open (liso.add_edge G x y u) ⩭ add_edge (open G) (inj_v x) u (inj_v y).
+Proof. 
+  have X : is_graph (add_edge (open G) (inj_v x) u (inj_v y)). 
+  { exact: add_edge_graph. }
+  rewrite /oliso. do 2 eexists.
+  apply: liso_comp (liso_sym _) _. apply: openK.
+  liso (imfset_bij (@inj_v_inj G)) 
+       (fresh_bij (imfset_bij (@inj_e_inj (edge G))))
+       (fun => false).
+  - move => v /=. by rewrite inj_vK.
+  - case => [e|] //=. 
+    + rewrite /update ifF ?inj_eK //. exact: fresh_imfsetF.
+    + by rewrite /update ifT.
+  - move => [e|]; apply: val_inj => /=;by rewrite /update /= ?fresh_imfsetF ?inj_eK // ifT.
+  - move => [e|]; apply: val_inj => /=;by rewrite /update /= ?fresh_imfsetF ?inj_eK // ifT.
+  - exact: val_inj.
+  - exact: val_inj.
+Defined.
+
+Lemma edges_at_open (x : G) (E : {set edge G}) :  
+  confluence.edges_at G x = E ->
+  edges_at (open G) (inj_v x) = [fset inj_e e | e in E].
+Admitted.
+
+Lemma oarc_open (x y : G) (e : edge G) u : 
+  arc G e x u y -> oarc (open G) (inj_e e) (inj_v x) u (inj_v y).
+Admitted.
+
+End Transfer.
 
 
+Lemma close_add_edge (G : pre_graph) (x y : VT) u 
+  (graph_G : is_graph G) (graph_G' : is_graph (add_edge G x u y)) : 
+  close (add_edge G x u y) ≅ liso.add_edge (close G) (proj_v (close G) x) (proj_v (close G) y) u.
+Proof.
+  apply: liso_sym. 
+  liso (bij_id) (fresh_bij bij_id) xpredT => //. 
+  4-5: exact: val_inj.
+Admitted.
   
+
+Lemma imfset1E (key : unit) (aT rT : choiceType) (f : aT -> rT) (x : aT) (A : finmempred aT) :
+  A =1 pred1 x -> imfset key f A = [fset f x].
+Admitted.
+Arguments imfset1E [key aT rT f] x [A].
+
+Lemma imfset_set1 (aT : finType) (rT : choiceType) (f : aT -> rT) (x : aT) : 
+  [fset f z | z in [set x]] = [fset f x].
+rewrite (imfset1E x) => //= z. by rewrite !inE. Qed.
+
+Lemma fsetDEl (T : choiceType) (A B : {fset T}) (x : A `\` B) : val x \in A.
+Proof. by case/fsetDP : (valP x). Qed.
+
+Definition bij_setD (aT : finType) (C : choiceType) (rT : {fset C}) (A : {set aT}) (f : bij aT rT) : 
+  bij { x | x \in ~: A} (rT `\` [fset val (f x) | x in A]).
+Proof.
+  set aT' := ({ x | _ }). set rT' := _ `\` _.
+  have g_proof (x : aT') : val (f (val x)) \in rT'.
+  { rewrite !inE (valP (f (val x))) andbT. apply: contraTN (valP x).
+    case/imfsetP => /= x0 inA /val_inj /(@bij_injective _ _ f) ->. by rewrite inE negbK. }
+  pose g (x : aT') : rT' := Sub (val (f (val x))) (g_proof x).
+  have g_inv_proof (x : rT') :  f^-1 (Sub (fsval x) (fsetDEl x)) \in ~: A.
+  { rewrite inE. case/fsetDP: (valP x) => ?. apply: contraNN => X. apply/imfsetP.
+    exists (f^-1 (Sub (fsval x) (fsetDEl x))) => //. by rewrite bijK'. }
+  pose g_inv (x : rT') : aT' := Sub (f^-1 (Sub (val x) (fsetDEl x))) (g_inv_proof x). 
+  have can1 : cancel g g_inv.
+  { move => [x Hx]. rewrite /g/g_inv. apply: val_inj => /=. apply: (@bij_injective _ _ f).
+    rewrite bijK'. exact: val_inj. }
+  have can2 : cancel g_inv g.
+  { move => [x Hx]. rewrite /g/g_inv. apply: val_inj => /=. by rewrite bijK'. }
+  apply: Bij can1 can2.
+Defined.
+
+
+(* TODO: use generic construction above *)
+Definition bij_delv (T : finType) (z : T) :  
+  bij { x:T | x \in [set~ z]} ([fset inj_v x | x in T] `\ inj_v z).
+Proof.
+  set A := ({ x | _ }). set B := _ `\ _.
+  have f_proof (x : A) : inj_v (val x) \in [fset inj_v x | x in T] `\ inj_v z by admit.
+  pose f (x : A) : B := Sub (inj_v (val x)) (f_proof x).
+  have f_inv_proof1 (x : B) : val x \in [seq inj_v z | z in [set~ z] ]. admit.
+  have f_inv_proof2 (x : B) : iinv (f_inv_proof1 x) \in [set~ z]. admit.
+  pose f_inv (x : B) := Sub (iinv (f_inv_proof1 x)) (f_inv_proof2 x) : A. simpl in *.
+  apply: (@Bij _ _ f f_inv).
+  - move => [x Hx]. rewrite /f_inv/f. apply: val_inj => /=. 
+    move: (f_inv_proof1 _) => /= H. rewrite in_iinv_f //. apply: in2W. exact: inj_v_inj.
+  - move => [x Hx]. rewrite /f_inv/f. apply: val_inj => /=. 
+Admitted.
+
+Lemma open_del_vertex (G : lgraph) (z : G) (Hz : z \notin IO) (Hz' : inj_v z \notin pIO (open G)) :
+  open (confluence.del_vertex G z Hz) ⩭ open G \ inj_v z.
+Proof.
+  eexists. unshelve eexists. eauto with typeclass_instances.
+  rewrite <- openK.
+  have B : bij (edge (confluence.del_vertex G z Hz)) (edge (close (open G \ inj_v z))) by admit.
+  liso (@bij_delv G z) B (fun _ => false).
+Admitted.
+
+(* Transfer the step relation *)
+
+Lemma ostep_of (G H : lgraph) :
+  step G H -> Σ H' : pre_graph, ostep (open G) H' * (H' ⩭ open H).
+Proof.
+  case => {G H}.
+  - move => G x z e Hz xDz u arc_e at_z. eexists; split.
+    + apply: ostep_v1. 3: apply: oarc_open arc_e.  
+      admit. admit. admit.
+    + 
+Admitted.
+
+(* TOTHINK: It appears that the "additive" variant of the step
+relation (i.e., the one that never deletes anything) is more
+convienient in the rest of the proofs. How reasonable is it to go
+directtly to the open removal variant, or do we want the removal
+variant on type-based graphs as intermediate representation? *)
